Update ActionsSemantics.thy, Auto_sep_record.thy, and 16 more files...

QSemantics.thy
@@ -5,7 +5,7 @@
 *)
 
 theory QSemantics
-  imports QSyntax vars "HOL-Library.Permutations" "List_Inversions.List_Inversions" "Tensor_Permutation"
+  imports QSyntax vars "HOL-Library.Permutations" "List_Inversions.List_Inversions"
 begin
 
 subsection \<open>Syntax\<close>
@@ -16,86 +16,80 @@ lemma "(1,2) \<in> inversions [0::nat,7,3,4] \<and> (1,3)\<in>inversions [0::nat
   by (simp add: inversions.simps) 
   
 
-type_synonym ('v,'b,'s,'q) QConf = "('v,'b,'s,'q) com \<times> ('s,'q) state"
-
-definition Q_domain::"'q::linorder q_vars \<Rightarrow> 'q set" 
-  where "Q_domain q_vars \<equiv> \<Union> (q_vars ` UNIV)"
-
-definition ket_dim ::"'q::linorder q_vars \<Rightarrow> nat"
-  where "ket_dim q_vars \<equiv>  card (Q_domain q_vars)"
-
-definition new_q_addr::"nat \<Rightarrow> 'q::linorder q_vars \<Rightarrow> ('q set) set"
-  where "new_q_addr n q_dom \<equiv> {s.  card s = n \<and> (Min s > Max (Q_domain q_dom))}"           
-
-lemma all_gt: "finite s' \<Longrightarrow> finite s \<Longrightarrow> 
-       Min s > Max s' \<Longrightarrow> (e::'q::linorder) \<in> s \<Longrightarrow> e' \<in> s' \<Longrightarrow> e > e'"
-  using Max_less_iff less_le_trans by fastforce
-
-lemma neq_q_addr_finites:"n\<noteq>0 \<Longrightarrow> S \<in> new_q_addr n q_dom \<Longrightarrow> finite S"
-  unfolding new_q_addr_def
-  using card_infinite by force
-
-lemma new_q_addr_gt_old_q_addr:
-  "n\<noteq>0 \<Longrightarrow> finite (Q_domain q_dom) \<Longrightarrow> 
-   S \<in> new_q_addr n q_dom \<Longrightarrow> e \<in> S \<Longrightarrow>
-   e' \<in> (Q_domain q_dom) \<Longrightarrow> e > e'"
-  unfolding new_q_addr_def using all_gt 
-  by (metis (mono_tags, lifting) card_infinite mem_Collect_eq)
-
-lemma new_q_addr_ortho_old_q_addr:
-  assumes a0:"n\<noteq>0" and a1:"finite (Q_domain q_dom)" and a2:"S \<in> new_q_addr n q_dom" 
-  shows "S \<subseteq> -(Q_domain q_dom)"
-proof - 
-  have f4: "card S = n \<and> Max (Q_domain q_dom) < Min S"
-    using a2 unfolding new_q_addr_def  by fastforce
-  then have "card S \<noteq> 0"
-    using a0 by meson
-  then have "finite S"
-    by (meson card_infinite)
-  then show ?thesis
-    using f4 a1 by (meson ComplI Max.coboundedI Min.coboundedI le_less_trans 
-                    less_le_not_le subsetI)
-qed 
- 
-definition list_dims::"'q::linorder set \<Rightarrow> nat list"
-  where "list_dims qvars \<equiv> replicate (card qvars) 2"
-
-definition dom_q_vars::"'q::linorder q_vars \<Rightarrow> nat set"
-  where "dom_q_vars q_vars \<equiv> Set.filter (\<lambda>e. q_vars e\<noteq>{}) UNIV"
-                                                  
-definition dims_heap::"'q::linorder q_vars \<Rightarrow> nat list"
-  where "dims_heap q_vars \<equiv> (list_dims o Q_domain) q_vars"
-
-definition qvars_lin_set::"'q::linorder q_vars \<Rightarrow> nat set"
-  where "qvars_lin_set q_vars \<equiv> {0 ..< (ket_dim q_vars)}"
-
-definition qvars_lin_sets::"'q::linorder q_vars \<Rightarrow> 'q::linorder q_vars \<Rightarrow> nat set"
-  where "qvars_lin_sets q_vars q_vars' \<equiv> {(ket_dim q_vars) ..< (ket_dim q_vars')}"
-
-definition sorted_list_from_set::"'q::linorder set \<Rightarrow> 'q::linorder list"
-  where "sorted_list_from_set s \<equiv> THE l. strict_sorted l \<and> set l = s"
-
 
 context vars
 begin
 
-
+(* m = partial_state2.ptensor_mat (dims_heap \<vv>) (q \<sigma>) ((Q_domain \<vv>)-(q \<sigma>)) (M::complex mat) (1\<^sub>m (card ((Q_domain \<vv>) - (q \<sigma>))))*)
 (* abbreviation "tensor_vec \<equiv> partial_state2.ptensor_vec" *)
+term  partial_state2.ptensor_mat
+
+definition apply_matrix_sep :: "'q::linorder set \<Rightarrow> ('q, complex) QState \<Rightarrow> complex mat \<Rightarrow> complex vec" 
+  where "apply_matrix_sep sep_vars qs M \<equiv>
+           let var_d = QState_vars qs in 
+           let v = QState_vector qs in
+           let t = sorted_list_of_set  sep_vars in
+           let l = sorted_list_of_set (var_d - sep_vars) in
+           let vs = sorted_list_of_set sep_vars in
+           let vs' = (t@l) in
+           let m = partial_state2.ptensor_mat (list_dims sep_vars @list_dims (var_d - sep_vars)) 
+                                        (lin_set sep_vars) (lin_sets (top_lin_set sep_vars) (var_d - sep_vars))
+                                        (M::complex mat) (1\<^sub>m (2^(card (var_d - sep_vars)))) in
+           let q = change_base vs v vs' in
+               change_base vs' (m *\<^sub>v q) vs
+        "
+
+definition alloc_vars :: "'q::linorder set \<Rightarrow> ('q, complex) QState \<Rightarrow> complex vec \<Rightarrow> complex vec"
+  where "alloc_vars sep_vars qs v \<equiv>            
+           partial_state2.ptensor_vec (list_dims (QState_vars qs)@list_dims sep_vars)
+                  (lin_set (QState_vars qs)) (lin_sets (top_lin_set ((QState_vars qs))) sep_vars)
+                  ( QState_vector qs) v"
+
+definition dispose_vars:: " 'q::linorder set \<Rightarrow> ('q, complex) QState \<Rightarrow> complex vec set"
+  where "dispose_vars sep_vars qs \<equiv> 
+   let vars_dom = QState_vars qs in
+   let v =   QState_vector qs in
+   let qv = (sorted_list_of_set vars_dom) in
+   let t = sorted_list_of_set sep_vars in
+   let l =  sorted_list_of_set (vars_dom - sep_vars) in
+   let qv' = t @ l in
+   let qn =  change_base qv v qv' in 
+   let vars_dom' = vars_dom \<union> sep_vars in
+    {q. (\<exists>q2. qn = partial_state2.ptensor_vec 
+                     ((list_dims vars_dom')@list_dims sep_vars)
+                     (lin_set vars_dom') (lin_sets (top_lin_set vars_dom') sep_vars ) 
+                      q q2)}"
+
+definition measure_vars::"nat \<Rightarrow>  'q::linorder set \<Rightarrow> ('q, complex) QState  \<Rightarrow> (real\<times>complex vec)"
+  where "measure_vars k  sep_vars qs \<equiv>
+   let vars_dom = QState_vars qs in
+    let v =   QState_vector qs in
+    let vars= (vars_dom - sep_vars) in
+    let l = (sorted_list_of_set sep_vars) in
+    let t = (sorted_list_of_set vars) in
+    let qv = (sorted_list_of_set vars_dom) in
+    let qv' = l @ t in 
+    let qn = change_base qv v qv' in
+    let mk = partial_state2.ptensor_mat (list_dims sep_vars @ list_dims vars)
+                 (lin_set sep_vars) (lin_sets (top_lin_set sep_vars) vars) (1\<^sub>k (2^(length l))) (1\<^sub>m (2^(length t))) in
+    let qn' =  mk  *\<^sub>v qn in 
+    let \<delta>k =  Re (((mat_adjoint (mat_of_rows (dim_vec v) [v]) *\<^sub>v qn') $ 0) div vec_norm qn') in    
+    let qnprod = ((sqrt \<delta>k)::complex) \<cdot>\<^sub>v qn' in
+       (\<delta>k, change_base qv' qnprod qv)" 
 
 inductive QSemantics::"'v set \<Rightarrow> ('v,'b,'s,'q::linorder) QConf \<Rightarrow> ('v,'b,'s,'q) QConf \<Rightarrow> bool" 
   ("_ \<turnstile> _ \<rightarrow> _" [81,81] 80) for \<Gamma>::"'v set" 
   where 
    StackMod:"\<Gamma> \<turnstile> (SMod f, (\<delta>,\<sigma>,\<Q>)) \<rightarrow> (Skip, (\<delta>,f \<sigma>,\<Q>))"
 
-| QMod:"(q \<sigma>)\<noteq>{} \<Longrightarrow> (q \<sigma>) \<subseteq> (Q_domain \<vv>) \<Longrightarrow> 
-         \<qq>' =  Normal_Tensor ((Q_domain \<vv>)-(q \<sigma>)) (Q_domain \<vv>) \<qq> \<Longrightarrow>
-         \<Gamma> \<turnstile> (QMod f q, (\<delta>,\<sigma>,(\<vv>,\<qq>))) \<rightarrow> (Skip, (\<delta>, \<sigma>,(\<vv>,\<qq>)))"
+| QMod:"(q \<sigma>)\<noteq>{} \<Longrightarrow> (q \<sigma>) \<subseteq> (QState_vars \<qq>) \<Longrightarrow> 
+         \<qq>' = apply_matrix_sep (q \<sigma>) \<qq> m \<Longrightarrow>
+         \<Gamma> \<turnstile> (QMod M q, (\<delta>,\<sigma>,(\<vv>,\<qq>))) \<rightarrow> (Skip, (\<delta>, \<sigma>,(\<vv>,QState(QState_vars \<qq>, list_of_vec  \<qq>'))))"
 
  | Alloc:"q' \<notin> (dom_q_vars \<vv>) \<Longrightarrow> q'_addr \<in> new_q_addr (e \<sigma>) \<vv> \<Longrightarrow> 
           \<vv>' = \<vv>(q' := q'_addr)  \<Longrightarrow> length (v \<sigma>) = (e \<sigma>) \<Longrightarrow> \<sigma>' = set_value \<sigma> q (nat_to_typ q') \<Longrightarrow>          
-          \<qq>' = partial_state2.ptensor_vec 
-                     (dims_heap \<vv>') (qvars_lin_set \<vv>') (qvars_lin_sets \<vv> \<vv>') (vec_of_list (v \<sigma>)) \<qq>  \<Longrightarrow>
-          \<Gamma> \<turnstile> (Alloc q e v, (\<delta>,\<sigma>,(\<vv>,\<qq>))) \<rightarrow> (Skip, (\<delta>, \<sigma>',(\<vv>',\<qq>')))"
+          \<qq>' = alloc_vars q'_addr \<qq> (vec_of_list (v \<sigma>)) \<Longrightarrow>
+          \<Gamma> \<turnstile> (Alloc q e v, (\<delta>,\<sigma>,(\<vv>,\<qq>))) \<rightarrow> (Skip, (\<delta>, \<sigma>',(\<vv>',QState(Q_domain \<vv>', list_of_vec  \<qq>'))))"
 
  | CondTrueQ:"\<sigma>\<in>b  \<Longrightarrow> \<Gamma> \<turnstile> (IF b c1 c2, (\<delta>,\<sigma>,\<Q>)) \<rightarrow> (c1, (\<delta>,\<sigma>,\<Q>))"
 
@@ -111,12 +105,15 @@ inductive QSemantics::"'v set \<Rightarrow> ('v,'b,'s,'q::linorder) QConf \<Righ
 
 | SeqSkipc: "\<Gamma>\<turnstile> (Skip;C2,\<sigma>) \<rightarrow> (C2, \<sigma>)"
 
- | Dispose: "\<vv> (q \<sigma>)\<noteq>{} \<Longrightarrow> \<vv>' = \<vv>((q \<sigma>):={}) \<Longrightarrow> 
-             \<qq>n = Normal_Tensor (\<vv> (q \<sigma>)) (Q_domain \<vv>) \<qq> \<Longrightarrow>
-             \<qq>n = partial_state2.ptensor_vec (dims_heap \<vv>) (qvars_lin_set \<vv>') (qvars_lin_sets \<vv>' \<vv>) \<qq>1 \<qq>2 \<Longrightarrow>  
-             \<Gamma> \<turnstile> (Dispose q, (\<delta>,\<sigma>,(\<vv>,\<qq>))) \<rightarrow> (Skip,(\<delta>,\<sigma>,(\<vv>',\<qq>1)))"
+| Dispose: "\<vv> (q \<sigma>) \<noteq> {} \<Longrightarrow> \<vv>' = \<vv>((q \<sigma>):={}) \<Longrightarrow> q1 ## q2  \<Longrightarrow> 
+            \<vv> (q \<sigma>) = QState_vars \<qq> \<Longrightarrow> \<qq> =   \<qq>1 +  \<qq>2 \<Longrightarrow>
+            \<qq>' \<in> dispose_vars (\<vv> (q \<sigma>)) \<qq> \<Longrightarrow>
+             \<Gamma> \<turnstile> (Dispose q, (\<delta>,\<sigma>,(\<vv>,\<qq>))) \<rightarrow> (Skip,(\<delta>,\<sigma>,(\<vv>',QState(Q_domain \<vv>', list_of_vec  \<qq>'))))"
 
- | Measure: "\<Gamma> \<turnstile> (Measure v qe, (\<delta>,\<sigma>,(\<vv>,\<qq>))) \<rightarrow> (Skip,(\<delta>,\<sigma>,(\<vv>',v1)))" 
+| Measure: "q \<sigma> \<subseteq> (Q_domain \<vv>) \<Longrightarrow> 
+            (\<delta>k, \<qq>') = measure_vars k (q \<sigma>) \<qq> \<Longrightarrow>
+            \<delta>k > 0 \<Longrightarrow> \<delta>' = \<delta> * \<delta>k \<Longrightarrow> 
+            \<Gamma> \<turnstile> (Measure v q, (\<delta>,\<sigma>,(\<vv>,\<qq>))) \<rightarrow> (Skip,(\<delta>',\<sigma>,(\<vv>',\<qq>')))" 
  
 
 
