QSyntax.thy
@@ -6,7 +6,7 @@
 
 
 theory QSyntax
-  imports HOL.Complex vars HOL.Orderings  QHLProver.Partial_State
+  imports HOL.Complex vars HOL.Orderings  QHLProver.Partial_State  Q_State
 begin                                             
 
 subsection \<open>Syntax\<close>
@@ -31,7 +31,8 @@ of the different variables, the vector dimension is the product of the size of e
 variable\<close> 
 
 type_synonym 'q q_vars = "(nat \<Rightarrow> 'q set)"
-type_synonym 'q qstate = "'q q_vars \<times> complex vec"
+type_synonym 'q qstate = "'q q_vars \<times> ('q, complex) QState"
+type_synonym 'q qheap = "'q set \<times> complex vec"
 type_synonym ('s,'q) state = "real \<times> 's \<times> 'q qstate"
 type_synonym 's pred = "'s \<Rightarrow> bool" 
 type_synonym 's assn = "'s set"
@@ -53,7 +54,96 @@ datatype ('a,'b,'s,'q::linorder) com =
   | Measure "'a"   "('s,'q) expr_q" ("_:=meassure / _" [60, 61] 60)
   | Alloc "'a"  "('s,nat) expr"  "('s,complex list) expr"  ("_:=alloc/[_/]/(_/)" [60, 61] 60)
   | Dispose "'s expr_nat" 
-                       
+
+type_synonym ('v,'b,'s,'q) QConf = "('v,'b,'s,'q) com \<times> ('s,'q) state"
+
+definition Q_domain::"'q::linorder q_vars \<Rightarrow> 'q set" 
+  where "Q_domain q_vars \<equiv> \<Union> (q_vars ` UNIV)"
+
+definition ket_dim ::"'q::linorder q_vars \<Rightarrow> nat"
+  where "ket_dim q_vars \<equiv>  card (Q_domain q_vars)"
+
+definition new_q_addr::"nat \<Rightarrow> 'q::linorder q_vars \<Rightarrow> ('q set) set"
+  where "new_q_addr n q_dom \<equiv> {s.  card s = n \<and> (Min s > Max (Q_domain q_dom))}"           
+
+lemma all_gt: "finite s' \<Longrightarrow> finite s \<Longrightarrow> 
+       Min s > Max s' \<Longrightarrow> (e::'q::linorder) \<in> s \<Longrightarrow> e' \<in> s' \<Longrightarrow> e > e'"
+  using Max_less_iff less_le_trans by fastforce
+
+lemma neq_q_addr_finites:"n\<noteq>0 \<Longrightarrow> S \<in> new_q_addr n q_dom \<Longrightarrow> finite S"
+  unfolding new_q_addr_def
+  using card_infinite by force
+
+lemma new_q_addr_gt_old_q_addr:
+  "n\<noteq>0 \<Longrightarrow> finite (Q_domain q_dom) \<Longrightarrow> 
+   S \<in> new_q_addr n q_dom \<Longrightarrow> e \<in> S \<Longrightarrow>
+   e' \<in> (Q_domain q_dom) \<Longrightarrow> e > e'"
+  unfolding new_q_addr_def using all_gt 
+  by (metis (mono_tags, lifting) card_infinite mem_Collect_eq)
+
+lemma new_q_addr_ortho_old_q_addr:
+  assumes a0:"n\<noteq>0" and a1:"finite (Q_domain q_dom)" and a2:"S \<in> new_q_addr n q_dom" 
+  shows "S \<subseteq> -(Q_domain q_dom)"
+proof - 
+  have f4: "card S = n \<and> Max (Q_domain q_dom) < Min S"
+    using a2 unfolding new_q_addr_def  by fastforce
+  then have "card S \<noteq> 0"
+    using a0 by meson
+  then have "finite S"
+    by (meson card_infinite)
+  then show ?thesis
+    using f4 a1 by (meson ComplI Max.coboundedI Min.coboundedI le_less_trans 
+                    less_le_not_le subsetI)
+qed 
+
+(* definition list_dims_set::"'q set \<Rightarrow> nat list"
+  where "list_dims_set qvars \<equiv> if qvars = {} then [1] 
+                            else replicate (card qvars) 2"
+
+definition list_dims::"'q::linorder set \<Rightarrow> nat list"
+  where "list_dims qvars \<equiv> replicate (card qvars) 2" *)
+
+definition dom_q_vars::"'q::linorder q_vars \<Rightarrow> nat set"
+  where "dom_q_vars q_vars \<equiv> Set.filter (\<lambda>e. q_vars e\<noteq>{}) UNIV"
+                                                  
+definition dims_heap::"'q::linorder q_vars \<Rightarrow> nat list"
+  where "dims_heap q_vars \<equiv> (list_dims o Q_domain) q_vars"
+
+definition qvars_lin_set::"'q::linorder q_vars \<Rightarrow> nat set"
+  where "qvars_lin_set q_vars \<equiv> {0 ..< (ket_dim q_vars)}"
+
+definition qvars_lin_sets::"'q::linorder q_vars \<Rightarrow> 'q::linorder q_vars \<Rightarrow> nat set"
+  where "qvars_lin_sets q_vars q_vars' \<equiv> {(ket_dim q_vars) ..< (ket_dim q_vars')}"
+
+(* definition top_lin_set::"'q set \<Rightarrow> nat" where
+  "top_lin_set qset \<equiv> if qset = {} then 1 else card qset"
+
+definition lin_set_alt::"'q set \<Rightarrow> nat set"
+  where "lin_set_alt qset \<equiv> if qset = {} then {0} else {0 ..< (card qset)}"
+
+definition lin_sets_alt::"nat \<Rightarrow> 'q set \<Rightarrow> nat set"
+  where "lin_sets_alt n q_vars' \<equiv> if q_vars' = {} then  {n}
+                                   else  {n ..< card (q_vars')}"
+
+definition lin_set::"'q::linorder set \<Rightarrow> nat set"
+  where "lin_set qset \<equiv> {0 ..< (card qset)}"
+
+definition lin_sets::"'q::linorder set \<Rightarrow> 'q::linorder set \<Rightarrow> nat set"
+  where "lin_sets q_vars q_vars' \<equiv> {card (q_vars) ..< card (q_vars')}"
+*)
+
+definition sorted_list_from_set::"'q::linorder set \<Rightarrow> 'q::linorder list"
+  where "sorted_list_from_set s \<equiv> THE l. strict_sorted l \<and> set l = s"
+
+definition to_heap::"'q::linorder qstate \<Rightarrow> ('q,complex) QState"
+  where "to_heap q \<equiv> snd q"
+
+
+
+definition projection1::"nat \<Rightarrow> nat \<Rightarrow> 'a::comm_ring_1 mat" ("1\<^sub>_ _") where
+  "projection1 k n \<equiv> mat n n (\<lambda> (i,j). if i = k \<and> j = k then 1 else 0)"
+
+
 locale h = vars + partial_state2 
 
 context vars 
