Tensor_Permutation.thy
@@ -18,6 +18,43 @@ definition list_permutations :: "'a list \<Rightarrow> 'a list set"
 definition permutes_lists::"'a list \<Rightarrow> 'a list \<Rightarrow> (nat \<Rightarrow> nat) set"
   where "permutes_lists ls ls' \<equiv> {p. p permutes {..<length ls} \<and> ls' = permute_list p ls}"
 
+lemma not_eq_length_no_permutation:
+  "length ls \<noteq> length ls' \<Longrightarrow> permutes_lists ls ls' = {}"
+  unfolding permutes_lists_def by auto
+
+lemma eq_length_there_is_perm:
+  "length ls = length ls' \<Longrightarrow> set ls = set ls' \<Longrightarrow> distinct ls \<Longrightarrow> 
+   permutes_lists ls ls' \<noteq> {}"
+  unfolding permutes_lists_def apply auto
+  by (metis card_distinct distinct_card mset_eq_permutation mset_set_set)
+
+lemma eq_perm_function: 
+  assumes    
+   a1:"p1 \<in> permutes_lists ls ls'" and
+   a2:"p2 \<in> permutes_lists ls ls'" and
+   a4:"distinct ls" 
+ shows "\<forall>n<length ls. p1 n = p2 n" 
+proof-
+  { fix n assume a00:"n < length ls"
+    have "ls' ! n = ls ! p1 n"
+      using a1 unfolding permutes_lists_def  
+      apply auto
+      by (metis (no_types)  a00 permute_list_nth)    
+    moreover have "ls' ! n = ls ! p2 n" 
+      using a2 unfolding permutes_lists_def  
+      apply auto
+      by (metis (no_types) a00 permute_list_nth)
+    ultimately have "ls ! p1 n = ls ! p2 n" by auto 
+    moreover have "p1 n < length ls"
+      using a1 a00  permutes_in_image permutes_lists_def 
+      by fastforce
+    moreover have "p2 n < length ls"
+      using a2 a00 permutes_in_image permutes_lists_def 
+      by fastforce
+    ultimately have "p1 n = p2 n" using a4 nth_eq_iff_index_eq by auto
+  }then show ?thesis by auto
+qed  
+
 definition list_permutations'::"'a list \<Rightarrow> 'a list set" where
   "list_permutations' ls = {ls'. \<exists>p. p permutes {..<length ls} \<and> ls' = permute_list p ls}"
 
@@ -36,17 +73,201 @@ lemma diff_permutations:
   unfolding list_permutations_def list_permutation_functions_def
   by force
 
+lemma "length (bin_to_bl l n) = l"
+  using Bits_Int.len_bin_to_bl by auto
+
+value "bl_to_bin (bin_to_bl 3 4)"
+
 definition permute_number :: "nat \<Rightarrow> (nat \<Rightarrow> nat) \<Rightarrow> nat \<Rightarrow>  nat"
   where "permute_number l p n \<equiv> nat (bl_to_bin (permute_list p (bin_to_bl l n)))"
+
+(* lemma permute_number_0:"permute_number 0 f = (\<lambda>n. 0)"
+  unfolding permute_number_def by auto *)
+
+lemma eq_bin_to_bl:
+  assumes a0:"\<forall>i<l. p i = i" 
+  shows "permute_list p (bin_to_bl l j) = (bin_to_bl l j)"
+    using a0 unfolding permute_list_def 
+    by (metis lessThan_atLeast0 lessThan_iff map_cong map_nth set_upt size_bin_to_bl) 
+
+lemma bl_to_bin_n_n:assumes a0:"(n::nat) < 2 ^ l" 
+  shows "bl_to_bin (bin_to_bl l n) = n"
+proof-
+  have "bl_to_bin (bin_to_bl l n) = bintrunc l n" 
+    using bin_bl_bin by auto
+  moreover have "bintrunc l n = n" using bintrunc_mod2p a0  by auto
+  ultimately show ?thesis  by auto 
+qed
+
+lemma permute_number_id: assumes a0:"\<forall>i<l. p i = i" and a1:"j < 2 ^ l" 
+    shows "(permute_number l p) j = j"
+proof-
+  have "permute_list p (bin_to_bl l j) = (bin_to_bl l j)"
+    using a0 eq_bin_to_bl by auto
+  moreover have  "bl_to_bin (bin_to_bl l j) = j" using bl_to_bin_n_n[OF a1] by auto    
+  ultimately show ?thesis unfolding permute_number_def 
+    by auto
+qed
+  
+  
+
+lemma eq_perm_func_eq_perm_list:
+  assumes a0:"\<forall>i<length l. p1 i = p2 i" and
+       a1:"p1 permutes {0..<length l}" and
+       a2:"p2 permutes {0..<length l}" 
+     shows "permute_list p1 l = permute_list p2 l"
+  using a0 a1 a2
+  by (metis length_permute_list lessThan_atLeast0 list_eq_iff_nth_eq permute_list_nth)
+
+lemma eq_permute_number:
+  assumes a0:"\<forall>i<l. p1 i = p2 i" and a1:"p1 permutes {0..<l}" and 
+          a2:"p2 permutes {0..<l}"  
+        shows "permute_number l p1 n = permute_number l p2 n"
+proof-
+  have "length (bin_to_bl l n) = l" 
+    using  Bits_Int.len_bin_to_bl by auto
+  then have "permute_list p1  (bin_to_bl l n) = permute_list p2  (bin_to_bl l n)"
+    using eq_perm_func_eq_perm_list a0 a1 a2 
+    by (auto intro:eq_perm_func_eq_perm_list)
+  thus ?thesis unfolding permute_number_def by auto
+qed
+
+lemma eq_permute_number2:
+  assumes a0:"\<forall>i<l. p1 i = p2 i" and a1:"p1 permutes {0..<l}" and 
+          a2:"p2 permutes {0..<l}"  
+        shows "(\<lambda>n. permute_number l p1 n) = (\<lambda>n. permute_number l p2 n)"
+  using a0 a1 a2 eq_permute_number by auto
 
 definition vector_permutation::"nat \<Rightarrow> 'a vec \<Rightarrow> (nat \<Rightarrow> nat) \<Rightarrow> 'a vec"
   where "vector_permutation n v p \<equiv>                                   
     vec_of_list (permute_list (permute_number n p)  (list_of_vec v))"
 
-definition Normal_Tensor::"'q::linorder set \<Rightarrow> 'q set \<Rightarrow> 'a vec \<Rightarrow> 'a vec"
-  where "Normal_Tensor q s v \<equiv> let l' = sorted_list_of_set (s-q)@(sorted_list_of_set q);
-                                p = SOME p. p \<in> permutes_lists (sorted_list_of_set s) l' in 
-                             vector_permutation (length l') v p"
+lemma eq_length:"l' = permute_list p l \<Longrightarrow> length l' = length l"
+  by auto
 
+lemma eq_vector_permutation: 
+  assumes a0:"distinct l" and  a1:"length l = length l'" and
+          a3:"p1 \<in>(permutes_lists l l')" and
+          a4:"p2 \<in>(permutes_lists l l')"
+  shows "vector_permutation (length l) v p1 = 
+         vector_permutation (length l) v p2"
+proof-
+  have "\<forall>n<length l. p1 n = p2 n" using eq_perm_function[OF a3 a4 a0] by auto
+  moreover have "length l = length l'"
+    using a3 not_eq_length_no_permutation by auto
+  ultimately have "permute_number (length l) p1 = permute_number (length l) p2"
+    using eq_permute_number  a3 a4 unfolding permutes_lists_def
+     by (metis (no_types, lifting) eq_permute_number2 lessThan_atLeast0 mem_Collect_eq)     
+  then show ?thesis
+    unfolding vector_permutation_def
+    by (simp add:  a1)
+qed
+
+lemma eq_vector_permutation_image_permutes:
+  assumes a0:"distinct l" and
+          a1:"x \<in> (vector_permutation (length l) v) ` (permutes_lists l l')" and
+          a2:"y \<in> (vector_permutation (length l) v) ` (permutes_lists l l')" 
+  shows "x = y"
+  using a0 a1 a2  
+  apply auto
+  apply (rule eq_vector_permutation[OF a0], auto)
+  using not_eq_length_no_permutation by blast
+
+definition change_orientation_set::"'q::linorder list \<Rightarrow> 'a vec \<Rightarrow> 'q list \<Rightarrow> 'a vec set"
+  where "change_orientation_set l v l' \<equiv>  
+     (vector_permutation (length l) v) ` (permutes_lists l l')"
+
+
+definition change_orientation::" 'a vec \<Rightarrow> 'q::linorder list \<Rightarrow> 'q list \<Rightarrow> 'a vec" ("_ . \<^sub>_ \<^sub>\<leadsto>  \<^sub>_" [80,80, 80] 80) 
+  where "change_orientation v l l' \<equiv>  
+     THE e. e \<in> change_orientation_set l v l'"
+
+lemma change_base_set_same_element:
+  assumes a0:"distinct l" and
+              a1:"x \<in> (change_orientation_set l v l')" and
+              a2:"y \<in> (change_orientation_set l v l')" 
+  shows "x = y"
+  using a0 a1 a2  unfolding change_orientation_set_def 
+  by (auto intro: eq_vector_permutation_image_permutes)
+
+lemma change_base_set_has_element:
+  assumes a0:"distinct l" and  a2:"length l = length l'" and 
+          a3:"set l = set l'"
+  shows "change_orientation_set l v l' \<noteq> {}"
+  using eq_length_there_is_perm[OF a2 a3 a0]  
+  unfolding change_orientation_set_def by auto
+
+lemma change_base_set_card_1:
+  assumes a0:"distinct l" and  a1:"length l = length l'" and 
+          a2:"set l = set l'"
+        shows "card (change_orientation_set l v l') = 1"
+  using change_base_set_same_element[OF a0] change_base_set_has_element[OF a0 a1 a2]  
+  by (metis is_singletonI' is_singleton_altdef)
+
+lemma change_base_alt_def: 
+  assumes a0:"distinct l" and  a1:"length l = length l'" and 
+          a2:"set l = set l'"
+  shows "(v.\<^sub>l\<^sub>\<leadsto>\<^sub>l') = 
+    vector_permutation (length l) v (SOME p. p \<in>(permutes_lists l l'))"  
+proof-
+  have "\<exists>p. p \<in>(permutes_lists l l')"
+    by (meson a0 a1 a2 all_not_in_conv eq_length_there_is_perm)
+  then show ?thesis unfolding change_orientation_set_def change_orientation_def
+    apply clarify
+    apply (rule the_equality)
+     apply (metis emptyE imageI some_in_eq)    
+    apply (erule imageE)             
+    using eq_vector_permutation[OF a0 a1] 
+          some_eq_ex[of "\<lambda>p. p \<in> permutes_lists l l'"]
+    by auto
+qed
+
+lemma change_orientation_length:
+  assumes a0:"distinct l" and  a1:"length l = length l'" and 
+          a2:"set l = set l'"
+        shows "dim_vec v  = dim_vec  (v.\<^sub>l\<^sub>\<leadsto>\<^sub>l')"  
+    unfolding change_base_alt_def[OF a0 a1 a2]
+              vector_permutation_def permute_list_def 
+    by auto
+
+lemma assumes a0:"i < length l" and 
+              a1:"p permutes {..<length l}" and 
+              a2:"l = map (\<lambda>i. l ! p i) [0..<length l]" and 
+              a3:"distinct l"
+            shows "p i = i"
+  using a0 a1 a2 a3
+  by (metis distinct_Ex1 lessThan_iff nth_mem permute_list_def permute_list_nth permutes_in_image)
+
+
+lemma eq_vector_same_permutation: 
+  assumes a0:"distinct l" and a1:"dim_vec v  = 2 ^ length l"
+  shows "v.\<^sub>l\<^sub>\<leadsto>\<^sub>l = v"
+proof-
+  have "\<forall>p \<in> permutes_lists l l. \<forall>i. i<(length l) \<longrightarrow> p i = i"
+    unfolding permutes_lists_def   using a0
+    apply auto     
+    by (metis distinct_Ex1 lessThan_iff nth_mem permute_list_nth permutes_in_image)
+  moreover have  "permutes_lists l l \<noteq> {}" using eq_length_there_is_perm a0 by auto  
+  ultimately obtain p where permutes:"p \<in> permutes_lists l l \<and> (\<forall>i. i<length l \<longrightarrow> p i = i)" by auto     
+  then   
+  have "dim_vec v = dim_vec (v.\<^sub>l\<^sub>\<leadsto>\<^sub>l)"    
+    by (metis a0 change_orientation_length)
+  moreover have  "(v.\<^sub>l\<^sub>\<leadsto>\<^sub>l)  = vector_permutation (length l) v p"  
+    using change_base_alt_def[OF a0] permutes eq_vector_permutation[OF a0]
+    by (smt someI_ex)
+  moreover have "\<forall>j< 2 ^ (length l). permute_number (length l) p j = j" 
+    using permutes permute_number_id by auto
+  then have "\<forall>i<dim_vec (v.\<^sub>l\<^sub>\<leadsto>\<^sub>l). v $ i = (v.\<^sub>l\<^sub>\<leadsto>\<^sub>l) $ i" using calculation
+    apply (auto simp add: vector_permutation_def)
+    by (simp add: a1 permute_list_def vec_of_list_index)    
+  ultimately show ?thesis by auto
+qed
+ 
+
+definition Normal_Tensor::"'q::linorder set \<Rightarrow> 'q set \<Rightarrow> 'a vec \<Rightarrow> 'a vec"
+  where "Normal_Tensor q s v \<equiv> 
+      let l' = sorted_list_of_set (s-q)@(sorted_list_of_set q);
+          p = SOME p. p \<in> permutes_lists (sorted_list_of_set s) l' in 
+        vector_permutation (length l') v p"
 
 end
