Q_State.thy
@@ -1,0 +1,565 @@
+theory Q_State
+  imports HOL.Complex vars HOL.Orderings  
+          Deep_Learning.Tensor_Matricization Separation_Algebra.Separation_Algebra
+          QHLProver.Partial_State Tensor_Permutation HOL.Finite_Set
+begin               
+
+definition list_dims::"'q set \<Rightarrow> nat list"
+  where "list_dims qvars \<equiv> replicate (card qvars) 2"
+
+definition top_lin_set::"'q set \<Rightarrow> nat" where
+  "top_lin_set qset \<equiv> if qset = {} then 1 else card qset"
+
+definition lin_set::"'q set \<Rightarrow> nat set"
+  where "lin_set qset \<equiv> if qset = {} then {0} else {0 ..< (card qset)}"
+
+definition lin_sets::"nat \<Rightarrow> 'q set \<Rightarrow> nat set"
+  where "lin_sets n q_vars' \<equiv> if q_vars' = {} then  {n}
+                                   else  {n ..< card (q_vars')+n}"
+
+\<comment>\<open> Lemmas on ptensor_vec \<close>
+
+lemma tensor_neutral:"partial_state.tensor_vec [] {} (vCons (1::'a::comm_ring_1) vNil) (vCons 1 vNil) = vCons 1 vNil "
+proof-
+ interpret ps2:partial_state "[]" "{}" .
+   
+  show ?thesis  unfolding ps2.tensor_vec_def unfolding  
+   ind_in_set_def partial_state.tensor_vec_def  state_sig.d_def 
+   partial_state.encode1_def partial_state.dims1_def 
+    partial_state.encode2_def partial_state.dims2_def  by auto
+qed
+
+lemma nths_set_gt_list_length:"nths l (- {0..<length l}) = []"
+proof -
+  have "nths l (- {0..<length l}) ! 0 \<notin> set (nths l (- {0..<length l}))"
+    by (simp add: set_nths)
+  then show ?thesis
+    by (meson length_greater_0_conv nth_mem)
+qed
+
+lemma digit_decode_non_vars:"digit_decode (nths (replicate (card d1) 2) (- {0..<card d1}))
+                  (nths (digit_encode (replicate (card d1) 2) i) (- {0..<card d1})) = 0"
+  using nths_set_gt_list_length
+  by (metis digit_decode.simps(1) length_digit_encode length_replicate)
+
+lemma digit_decode_vars:
+   "i< (2::nat) ^ card (d1) \<Longrightarrow> 
+    digit_decode (nths (replicate (card d1) 2) {0..<card d1})
+                 (nths (digit_encode (replicate (card d1) 2) i) {0..<card d1}) = i"  
+  by (simp add: length_digit_encode nths_all)
+  
+lemma list_of_neutral:"list_of_vec (vCons 1 vNil) = [1::'a::comm_ring_1]"
+  unfolding vCons_def by auto  
+
+lemma list_ptensor_neutral:"list_of_vec
+       (partial_state.tensor_vec [] {}
+       (vCons (1::'a) vNil) (vCons (1::'a::comm_ring_1) vNil)) =
+       [1::'a::comm_ring_1]"
+  by (auto simp add: tensor_neutral list_of_neutral)
+
+lemma idempoten_qstate1: 
+  assumes 
+    a0:"dim_vec (v::('a::comm_ring_1) vec) = (2::nat) ^ card (d1)" and
+    a1:"i < dim_vec v"
+  shows 
+     "partial_state.tensor_vec (replicate (card d1) (2::nat))
+             {0::nat..<card  d1} v (vCons 1 vNil) $ i = 
+         v $ i"
+proof-
+  interpret ps2:partial_state "(replicate (card d1) (2::nat))" "{0::nat..<card  d1}" .
+  let  ?d0 = "digit_decode (nths (replicate (card d1) 2) (- {0..<card d1}))
+                  (nths (digit_encode (replicate (card d1) 2) i) (- {0..<card d1}))"
+  have vcons_0:"vCons 1 vNil $ ?d0 = 1" by  (auto simp add: digit_decode_non_vars)
+  moreover have  "digit_decode (nths (replicate (card d1) 2) {0..<card d1})
+                 (nths (digit_encode (replicate (card d1) 2) i) {0..<card d1}) = i" 
+    using digit_decode_vars a0 a1 by auto
+  moreover have " (prod_list (replicate (card d1) 2)) = (2::nat) ^ card (d1)" by auto
+  ultimately show ?thesis unfolding ps2.tensor_vec_def 
+      partial_state.tensor_vec_def state_sig.d_def partial_state.encode1_def 
+      partial_state.encode2_def partial_state.dims1_def partial_state.dims2_def     
+    using a1 a0   apply clarsimp  by (auto simp add: vcons_0)
+    
+qed
+
+lemma nths_a_as1:
+     "nths (n # replicate m n) {0..(Suc m)} = 
+       n # (nths (replicate m n) {0..< (m)})"  
+proof (induct m)
+  case 0
+  then show ?case by auto
+next
+  case (Suc m)
+  then show ?case
+    by (simp add: nths_all)
+qed 
+  
+lemma nths_a_as:
+     "nths (n # replicate m n) (insert (Suc m) {0..<Suc m}) = 
+       n # (nths (replicate m n) (insert m {0..< m}))"  
+proof-
+  have "nths (n # replicate m n) (insert (Suc m) {0..<Suc m}) = 
+        nths (n # replicate m n) {0..<Suc (Suc m)}"
+    using set_upt_Suc by presburger
+  moreover have "n # (nths (replicate m n) (insert m {0..< m})) = 
+                 n # (nths (replicate m n) {0..< Suc m})"
+    using set_upt_Suc by presburger
+  ultimately show ?thesis using nths_a_as1
+    by (simp add: atLeast0LessThan)
+qed
+
+lemma prod_list_dims_eq_2_pow_card_a:
+   "finite (d1) \<Longrightarrow> d1 \<noteq> {} \<Longrightarrow>    
+    prod_list
+     (nths (replicate (card d1) (2::nat))
+       (insert (card d1) {0..<card  d1})) = 2 ^ card d1"
+proof(induct "d1" rule:finite_induct)
+  case empty
+  then show ?case by auto
+next
+  case (insert x F)
+  { assume a00:"F = {}" 
+    then have "insert x F = {x}" using insert by auto
+    then have "card  {x} = 1"
+      by (simp add: card_1_singleton_iff)
+    moreover have "prod_list (nths (replicate 1 (2::nat)) {0,1}) = 2 ^ card  {x}"
+      using calculation by auto
+    ultimately have ?case
+      by (simp add: a00)
+  }
+  moreover { 
+    assume F:"F\<noteq> {}"
+    have "x \<notin> F" using insert by auto    
+    then have "prod_list (nths (replicate (card F) (2::nat)) (insert (card F) {0..<card F})) = 
+               2 ^ card F" using insert(3)[OF F] by auto    
+    then have ?case using insert(4)
+      by (simp add: nths_all)             
+  }
+  ultimately show ?case
+    by blast
+qed
+
+
+lemma idempoten_qstate2: 
+  assumes 
+    a1:"dim_vec v = (2::nat) ^ card d " and a2:"finite d"
+  shows "dim_vec
+     (partial_state.tensor_vec (replicate (card d) 2)
+       {0::nat..<card  d} v (vCons 1 vNil)) =
+      dim_vec v"
+proof-
+  interpret ps2:partial_state "(replicate (card d) (2::nat))" 
+                               "{0::nat..<card d}" .
+  show ?thesis unfolding ps2.tensor_vec_def  
+      partial_state.tensor_vec_def state_sig.d_def partial_state.encode1_def 
+      partial_state.encode2_def partial_state.dims1_def vCons_def 
+    using a1 by auto
+qed
+
+lemma idempoten_qstate:
+  assumes 
+    a1:"dim_vec (v::('a::comm_ring_1) vec) = (2::nat) ^ card d" and a2:"finite d"
+  shows "partial_state.tensor_vec (list_dims d)  {0::nat..<card d} v (vCons (1) vNil) = v"
+  unfolding list_dims_def using idempoten_qstate1[OF a1] idempoten_qstate2[OF  a1 a2]
+  using a2 by blast
+
+
+
+typedef (overloaded) ('q,'a::comm_ring_1)
+  QState = "{(s,v)| (s::'q set) (v::'a list).                                   
+              length v = (2^(card s)) \<and> finite s \<and>
+              (s = {} \<longrightarrow> ((v!0) = (1::'a)))}"
+  morphisms uQState Abs_QState  
+  by (rule exI[where x ="({},[1])"], auto)
+
+setup_lifting type_definition_QState
+
+definition tensor_mat_ord::"('q,'a)QState \<Rightarrow> 'q set \<Rightarrow> 'a::comm_ring_1 mat \<Rightarrow> ('q,'a)QState set"
+  where "tensor_mat_ord Q q M \<equiv> {}"
+
+lemma QState_rel1:"length(snd(uQState x)) = 2 ^ card (fst(uQState x))"  
+proof -
+  have "\<exists>B v. uQState x = (B, v) \<and> length v = (2 ^ card B) \<and> 
+              (B = {}) \<longrightarrow> (v ! 0 = 1)"
+    using uQState by fastforce
+  then show ?thesis using uQState  by (auto simp add:  split_beta)    
+qed
+
+lemma QState_rel2:"fst (uQState (x::('q,'a::comm_ring_1) QState )) = {} \<longrightarrow> 
+                  (((snd (uQState x)) ! 0) = 1)"
+proof -
+  have "\<exists>B v. uQState x = (B, v) \<and> length v = (2 ^ card B) \<and> 
+              (B = {}) \<longrightarrow> (v ! 0 = 1)"
+    using uQState by fastforce
+  then show ?thesis using uQState  by (auto simp add:  split_beta)       
+qed
+
+lemma QState_rel3:"finite (fst (uQState (x::('q,'a::comm_ring_1) QState )))"
+  apply transfer by auto
+ 
+lift_definition QState_vars :: "('q,'a::comm_ring_1) QState \<Rightarrow> 'q set" is fst .
+lift_definition QState_list :: "('q,'a::comm_ring_1) QState \<Rightarrow> 'a::comm_ring_1 list" is snd .
+lift_definition QState_vector::"('q,'a::comm_ring_1) QState \<Rightarrow> 'a::comm_ring_1 vec" is "\<lambda>s. vec_of_list (snd s)" .
+lift_definition QState :: "'q set \<times> 'a::comm_ring_1 list \<Rightarrow> ('q,'a)QState" is  
+  "\<lambda>s. (if fst s = {} \<and> snd s = [1] then (fst s, snd s)
+       else (if finite (fst s) \<and> fst s \<noteq> {} \<and> length (snd s) = 2 ^ (card (fst s)) then (fst s, snd s)
+       else ({}, [1])))"  by auto
+
+lift_definition Conc :: " ('q,'a) QState \<Rightarrow> 'q set \<times> 'a::comm_ring_1 vec" is
+  "\<lambda>s. (QState_vars s, QState_vector s)" .
+
+lemma uqstate_fst:"fst (uQState a) = QState_vars a" apply transfer' by auto
+lemma uqstate_snd:"snd (uQState a) = QState_list a" apply transfer' by auto
+
+lemma QState_rel3':"finite (QState_vars (x::('q,'a::comm_ring_1) QState ))"
+  apply transfer by auto
+
+lemma QState_rel1':"length(QState_list x) = 2 ^ card (QState_vars x)"
+  using uqstate_fst uqstate_snd  QState_rel1
+  by metis 
+
+lemma QState_rel2':"QState_vars x = {} \<Longrightarrow> 
+                  (((QState_list x) ! 0) = 1)"
+using uqstate_fst uqstate_snd  QState_rel2
+  by metis 
+
+lemma QState_empty0:"QState_vars x = {} \<Longrightarrow> 
+                     QState_list x = [1]"
+  apply (frule QState_rel2'[of x]) apply (insert QState_rel1'[of x])
+  apply auto
+  by (metis Suc_length_conv list_exhaust_size_eq0 nth_Cons_0)
+
+lemma QState_empty1:"QState_list x = [1] \<Longrightarrow> QState_vars x = {}"
+  using QState_rel1' QState_rel3'
+  by (metis One_nat_def card_eq_0_iff length_Cons list.size(3) nat_power_eq_Suc_0_iff 
+     numeral_eq_one_iff semiring_norm(85)) 
+
+lemma QState_empty:"QState_vars x = {} = ((QState_list x) = [1])"
+  using QState_empty1 QState_empty0 by auto
+
+
+lemma uQState_fst_id_concat:"fst (uQState a) \<union> fst (uQState (QState ({}, [1]))) = fst (uQState a)"
+  by (simp add: QState.rep_eq)
+
+lemma QState_vars_id:"QState_vars a \<union> QState_vars (QState ({},[1])) = QState_vars a"
+  by (simp add: uqstate_fst[THEN sym] uQState_fst_id_concat)  
+
+lemma fst_uQState_empty: "fst (uQState (QState ({}, [1]))) = {}"
+  apply transfer by auto
+
+lemma snd_uQState_empty: "snd (uQState (QState ({}, [1]))) = [1]"
+  apply transfer by auto
+
+lemma q_state_eq:
+ "a = b = 
+ (QState_vars a = QState_vars b \<and> QState_list a = QState_list b)"
+  apply transfer by auto
+
+
+lemma QState_id_fst_empty:
+    "a = QState ({}, [1]) \<Longrightarrow>
+    fst (uQState a) = {}"
+  apply transfer by auto
+
+lemma fst_uQState_empty_snd_1:"a \<noteq> QState ({}, [1]) \<Longrightarrow>
+       fst (uQState a) = {} \<Longrightarrow> snd (uQState a) = [1]"
+  apply (cases "QState_vars a \<noteq> {} \<and> length (QState_list a) = 2^(card (QState_vars a)) ")
+  apply transfer'
+   apply (simp add: QState_list.rep_eq QState_rel1 QState_vars.rep_eq)
+  apply transfer apply auto using  List.list_eq_iff_nth_eq by fastforce
+
+
+lemma fst_uQState_not_empty_wf_uQState:"fst (uQState a) \<noteq> {} \<Longrightarrow> 
+      length (snd (uQState a)) =  2^(card (fst (uQState a)))"
+  apply transfer by auto
+
+lemma QState_refl:"QState (QState_vars a, QState_list a) = a"
+  apply transfer apply auto using List.list_eq_iff_nth_eq by fastforce
+
+lemma "QState_vars (QState (QState_vars a, QState_list a)) = QState_vars a"
+  by (simp add:  QState_refl)
+
+lemma "QState_list (QState (QState_vars a, QState_list a)) = QState_list a"
+  by (simp add:  QState_refl)
+
+value "digit_decode [2,2,2] (nths (digit_encode [2,2,2,2] 9) {0,1,2})"
+\<comment>\<open>Definition of plus_QState_vector\<close>
+value "nths [2::nat,2,2] {(4::nat),5}"
+value "(digit_encode [2,2,2,2] 9)"
+value "nths (digit_encode [2,2,2,2] 9) {3}"
+value "digit_decode [2] (nths (digit_encode [2,2,2,2] 9) {3})"
+  
+definition plus_QState_vector::"('q::linorder,'a::comm_ring_1) QState \<Rightarrow> ('q,'a::comm_ring_1) QState \<Rightarrow>'q set \<times> 'a::comm_ring_1 list"
+  where "plus_QState_vector q1 q2 \<equiv> 
+     let d1 = (QState_vars q1); d2 = (QState_vars q2); 
+          s = d1 \<union> d2; l1 = QState_vector q1; l2 = QState_vector q2;
+          dims = list_dims s;  
+          v = partial_state.tensor_vec 
+                     dims {0..<card d1} l1 l2;
+          a = ((sorted_list_of_set d1)@(sorted_list_of_set d2));
+          b = sorted_list_of_set s in (s, list_of_vec (v.\<^sub>a \<^sub>\<leadsto> \<^sub>b))"
+
+lemma QState_vars_empty:"QState_vars (QState ({}, [1])) = {}"
+  by (metis (no_types) QState_id_fst_empty uqstate_fst)
+  
+
+lemma plus_QState_vector_a_idem:
+  "snd (plus_QState_vector a (QState ({}, [1]))) = QState_list a"  
+proof-
+  let ?v0 = "QState ({}, [1])::('b, 'a) QState"  
+  let ?s0 = "sorted_list_of_set (QState_vars ?v0)"
+  let ?b = "sorted_list_of_set (QState_vars a)"
+  let ?a = "?b @ ?s0" 
+  have card_vars_a:"dim_vec (QState_vector a) = 2^card (QState_vars a)"
+    by (simp add: QState_rel1' QState_vector.rep_eq uqstate_snd)
+  moreover have finite_vars_a:"finite (QState_vars a)"
+    by (simp add: QState_rel3')
+  ultimately have 
+    tensor_prod:"partial_state.tensor_vec (list_dims (QState_vars a))  {0::nat..<card ((QState_vars a))} 
+                                (QState_vector a) (vCons (1) vNil) = QState_vector a"
+    using idempoten_qstate by fastforce
+  have  vars_v0:"QState_vars ?v0 = {}"
+    by (simp add: QState_vars.rep_eq fst_uQState_empty)
+  have  v0:"QState_vector ?v0 = vCons (1::'a::comm_ring_1) vNil"
+    by (simp add: QState_vector.rep_eq snd_uQState_empty)
+  have  s:"(QState_vars a) \<union> (QState_vars ?v0) = (QState_vars a)"
+    by (simp add: QState_vars_id)
+  then have  "sorted_list_of_set ((QState_vars a) \<union> (QState_vars ?v0)) = sorted_list_of_set (QState_vars a)"
+    by metis
+  moreover have  "sorted_list_of_set (QState_vars a)@sorted_list_of_set (QState_vars ?v0) = 
+              sorted_list_of_set (QState_vars a)"
+    by (simp add: vars_v0)
+  then have  "QState_vector a = (QState_vector a).\<^sub>?a \<^sub>\<leadsto> \<^sub>?b"
+    using eq_vector_same_permutation
+    by (metis card_vars_a finite_vars_a distinct_card 
+        distinct_sorted_list_of_set sorted_list_of_set(1))    
+  then show ?thesis unfolding plus_QState_vector_def Let_def
+     using s v0 tensor_prod   apply transfer'
+     by (simp add: list_vec )
+qed
+
+definition plus_QState:: "('q::linorder,'a::comm_ring_1) QState \<Rightarrow> ('q,'a::comm_ring_1) QState \<Rightarrow> ('q,'a::comm_ring_1) QState"
+  where "plus_QState q1 q2 \<equiv> 
+    let d1 = (QState_vars q1); d2 = (QState_vars q2) in
+      if (d1 \<inter> d2 \<noteq> {}) then QState ({},[1])
+      else QState (plus_QState_vector q1 q2)"
+
+definition disj_QState::"('q,'a::comm_ring_1) QState \<Rightarrow> ('q,'a::comm_ring_1) QState \<Rightarrow> bool"
+  where "disj_QState q1 q2 \<equiv> QState_vars q1 \<inter> QState_vars q2 = {}"
+
+(* lift_definition disj_QState :: "('q,'a::comm_ring_1) QState \<Rightarrow> ('q,'a::comm_ring_1) QState \<Rightarrow> bool" is
+  "\<lambda>a b. fst a \<inter> fst b = {}" . *)
+
+\<comment>\<open>Lemmas on plus_QState_vector\<close>
+
+\<comment>\<open>plus_QState_vector is well formed: 
+   the set of vars is finite, the length of the product tensor is 2^ of the cardinality of the vars
+   if the set of vars is empty, then the tensor is [1]
+\<close>
+
+lemma plus_QState_set_wf:"\<lbrakk>d1 = (QState_vars q1); d2 = (QState_vars q2);
+          s = d1 \<union> d2\<rbrakk> \<Longrightarrow> finite s"
+  apply transfer by fastforce
+
+lemma plus_QState_vector_set_wf:"finite (fst (plus_QState_vector q1 q2))"
+  unfolding plus_QState_vector_def Let_def using plus_QState_set_wf
+  by fastforce 
+
+lemma prod_list_card_d_empty_one:" d\<noteq>{} \<Longrightarrow>
+       prod_list (nths (replicate (card d) 2) {0..<Suc (card d)}) = 2 ^ card d"
+  by (metis atLeast0LessThan length_replicate lessI lessThan_iff 
+           less_trans nths_all prod_list_replicate)
+
+
+lemma dim_vec_plus_2_pow_s:
+  assumes a0:"d1 = QState_vars q1" and a1:"d2 = QState_vars q2" and
+          a2:"s = d1 \<union> d2" and a3:"l1 = QState_vector q1" and a4:"l2 = QState_vector q2" and
+          a5:"ds = list_dims s" and
+          a6:"v = partial_state.tensor_vec 
+                     ds  {0..<card d1} l1 l2"  and a7:"d1 \<inter> d2 = {}"
+  shows "dim_vec v = (2^(card s))"
+proof-
+  interpret ps2:partial_state ds  "{0..<card d1}" .
+  have "dim_vec l1 = 2^card d1" 
+    using a0  QState_rel1'[of q1] a3 apply transfer' by auto
+  moreover have "dim_vec l2 = 2^card d2" 
+    using a1  QState_rel1'[of q2] a4 apply transfer' by auto
+  moreover have "finite d2"
+    by (simp add: QState_rel3' a1)
+  moreover have "finite d1" by (simp add: QState_rel3' a0)
+  ultimately have "dim_vec v = prod_list ds"
+    using a6  a5 a7 a2 unfolding ps2.tensor_vec_def   
+  partial_state.tensor_vec_def  state_sig.d_def 
+   partial_state.encode1_def partial_state.dims1_def 
+    partial_state.encode2_def partial_state.dims2_def by auto
+  thus ?thesis using a5 unfolding list_dims_def by auto
+qed    
+  
+
+lemma plus_QState_vector_wf':
+  assumes a9:"d1 \<inter> d2 = {}" and
+          a0:"d1 = (QState_vars q1)" and a1:"d2 = (QState_vars q2)" and
+          a2:"s = d1 \<union> d2" and a3:"l1 = QState_vector q1" and a4:"l2 = QState_vector q2" and
+          a5:"ds = list_dims s" and
+          a6:"v = partial_state.tensor_vec ds  {0..<card d1} l1 l2" and
+          a7:"a = ((sorted_list_of_set d1)@(sorted_list_of_set d2))" and
+          a8:"b = sorted_list_of_set s" 
+        shows "length (list_of_vec (v.\<^sub>a \<^sub>\<leadsto> \<^sub>b)) =  (2^(card s))"
+proof-
+  have "dim_vec v = (2^(card s))" using dim_vec_plus_2_pow_s[OF a0 a1 a2 a3 a4 a5 a6 a9] by auto
+  moreover have "distinct a"
+    using QState_rel3' a0 a1 a7 a9 set_sorted_list_of_set by auto
+  moreover have "length a = length b"
+    by (metis QState_rel3' a0 a1 a2 a7 a8 a9 card_Un_disjoint distinct_card 
+              distinct_sorted_list_of_set finite_UnI length_append set_sorted_list_of_set)
+  moreover have "set a = set b"
+    by (simp add: QState_rel3' a0 a1 a2 a7 a8)
+  ultimately show ?thesis using change_orientation_length
+    by (metis length_list_of_vec)
+qed        
+
+lemma plus_QState_vector_wf: assumes a0: "QState_vars q1 \<inter> QState_vars q2 = {}"
+  shows "length (snd (plus_QState_vector q1 q2)) =
+        2 ^ card (fst (plus_QState_vector q1 q2))"
+  unfolding plus_QState_vector_def Let_def using a0
+  apply clarsimp apply (frule plus_QState_vector_wf')  
+  by force+
+
+lemma plus_QState_vector_empty_vars_one_wf:
+  assumes a0:"fst (plus_QState_vector q1 q2) = {} " 
+  shows "snd (plus_QState_vector q1 q2) = [1]"
+proof-
+  have "QState_vars q1 = {} \<and> QState_vars q2 = {}"
+    using a0 unfolding plus_QState_vector_def Let_def by  auto
+  moreover have "QState_list q1 = [1] \<and> QState_list q2 = [1]" 
+    using QState_empty calculation
+    by auto  
+  ultimately show ?thesis 
+    unfolding plus_QState_vector_def Let_def list_dims_def  
+    apply auto apply transfer'
+    by (simp add: eq_vector_same_permutation tensor_neutral)
+qed                                             
+
+ 
+lemma QState_vars_Plus:"(QState_vars q1 \<inter> QState_vars q2 \<noteq> {} \<longrightarrow>
+          QState_vars (plus_QState q1 q2) = {}) \<and>        
+       (QState_vars q1 \<inter> QState_vars q2 = {} \<longrightarrow> 
+           QState_vars (plus_QState q1 q2) = fst (plus_QState_vector q1 q2))"  
+    apply (auto simp add: plus_QState_def ) apply transfer
+    apply simp 
+   apply transfer' using plus_QState_vector_set_wf plus_QState_vector_wf  
+   apply (smt fst_conv)
+   apply transfer' using plus_QState_vector_set_wf plus_QState_vector_wf
+  by fastforce
+
+lemma QState_list_Plus:"(QState_vars q1 \<inter> QState_vars q2 \<noteq> {} \<longrightarrow>
+          QState_list (plus_QState q1 q2) = [1]) \<and>        
+       (QState_vars q1 \<inter> QState_vars q2 = {} \<longrightarrow> 
+           QState_list (plus_QState q1 q2) = snd (plus_QState_vector q1 q2))"  
+    apply (auto simp add: plus_QState_def ) apply transfer
+    apply auto
+  apply transfer 
+  apply auto 
+  using plus_QState_vector_set_wf plus_QState_vector_wf plus_QState_vector_empty_vars_one_wf
+  by  blast+
+
+lemma neutral_vector_wf:"length [1] = (2^(card {}))" by auto
+
+lemma plus_QState_finite:"finite (QState_vars (plus_QState q1 q2))"  
+  by (simp add: QState_rel3')
+
+lemma plus_QState_length:"length (QState_list (plus_QState q1 q2)) =  2^card (QState_vars (plus_QState q1 q2))"  
+  by (simp add: QState_rel1')
+
+lemma plus_QState_neutral:
+  "QState_vars (plus_QState q1 q2) = {} = 
+   ((QState_list (plus_QState q1 q2)) = [1])"  
+  using QState_empty by auto
+
+
+
+(* lift_definition plus_QState :: "('q,'a::comm_ring_1) QState \<Rightarrow> ('q,'a::comm_ring_1) QState \<Rightarrow> ('q,'a::comm_ring_1) QState" is  
+  "\<lambda>a b. let d1 = fst a; d2 = fst b; s = d1 \<union> d2; l1 = snd a; l2 = snd b;
+             dims = list_dims s;
+              v = partial_state2.ptensor_vec 
+                     dims (lin_set d1) (lin_sets (top_lin_set d1) d2) 
+                         (vec_of_list l1)  (vec_of_list l2) in
+                  QState (s,list_of_vec v)" . *)
+
+
+(* lemma uQState_fst_id_ptensor:"
+       (partial_state.tensor_vec (list_dims (d \<union> {}))
+          {0..<card d1}  v (vCons 1 vNil)) = v"  
+  unfolding list_dims_def lin_set_def lin_sets_def top_lin_set_def apply auto
+  using list_ptensor_neutral apply blast  
+  apply (fastforce simp add: fst_uQState_empty_snd_1 list_ptensor_neutral) sorry
+  by (metis QState_rel1 dim_vec_of_list equals0D idempoten_qstate list_vec) *)
+
+
+lemma plus_idem:"plus_QState a (QState ({},[1])) = a"
+proof-
+  {
+    assume a00:"QState_vars a = {}"
+    have ?thesis
+      by (metis (no_types, lifting) QState_empty QState_refl 
+          QState_vars_Plus QState_vars_id a00 fst_conv plus_QState_vector_def) 
+  }
+  moreover {
+    let ?n = "QState ({},[1])"
+    assume a00:"QState_vars a \<noteq>{}"
+    have "fst (plus_QState_vector a ?n) = QState_vars a"
+      by (metis QState_vars_id fst_conv plus_QState_vector_def)
+    moreover have "snd (plus_QState_vector a ?n) = QState_list a"
+      by (simp add: plus_QState_vector_a_idem)
+    moreover have "QState_vars (plus_QState a ?n) = fst (plus_QState_vector a ?n) "
+      using QState_vars_Plus
+      by (metis fst_uQState_empty inf_bot_right uqstate_fst)
+    moreover have "QState_list (plus_QState a ?n) = snd (plus_QState_vector a ?n)"            
+      by (simp add: QState_list_Plus QState_vars.rep_eq fst_uQState_empty)
+    ultimately have ?thesis using q_state_eq by auto
+  }
+  ultimately show ?thesis by auto 
+qed
+
+
+lemma plus_comm:"disj_QState x y \<Longrightarrow> plus_QState x y = plus_QState y x"
+proof-
+  assume "disj_QState x y"
+  then have "QState_vars x  \<inter> QState_vars y = {}"
+    unfolding disj_QState_def by auto
+  show "plus_QState x y = plus_QState y x"
+    sorry
+qed
+
+lemma plus_assoc:" \<lbrakk>disj_QState x y; disj_QState y z; disj_QState x z\<rbrakk>
+       \<Longrightarrow> plus_QState (plus_QState x y) z = plus_QState x (plus_QState y z)"
+  sorry
+
+
+lemma plus_disj_dist:"\<lbrakk>disj_QState x (plus_QState y z); disj_QState y z\<rbrakk> \<Longrightarrow> disj_QState x y"
+  sorry
+
+lemma plus_dis_dist2:" \<lbrakk>disj_QState x (plus_QState y z); disj_QState y z\<rbrakk> \<Longrightarrow> disj_QState (plus_QState x y) z"
+  sorry
+
+
+
+instantiation QState :: (linorder,comm_ring_1) sep_algebra
+begin
+definition zero_QState: "0 \<equiv> QState ({},[1])"
+definition plus_QState: "s1 + s2 \<equiv> plus_QState s1 s2" 
+definition sep_disj_QState: "s1 ## s2 \<equiv> disj_QState s1 s2"
+instance 
+  apply standard
+  apply (simp add: zero_QState sep_disj_QState)
+        apply transfer'  apply auto         
+       apply (simp add: zero_QState sep_disj_QState) 
+       apply transfer apply auto 
+      apply (auto simp add: zero_QState  plus_QState Let_def intro:plus_idem)[1]
+     apply (auto simp add: sep_disj_QState plus_QState intro:plus_comm)[1]
+    apply (auto simp add: sep_disj_QState plus_QState intro:plus_assoc)[1]
+   apply (auto simp add: sep_disj_QState plus_QState intro:plus_disj_dist)[1]
+  apply (auto simp add: sep_disj_QState plus_QState intro:plus_dis_dist2)[1]
+  done
+end
+
+end
