Sep_Algebra_QState.thy
@@ -1,0 +1,10 @@
+theory Sep_Algebra_QState
+  imports  Separation_Algebra.Separation_Algebra
+begin                                      
+instantiation prod :: (zero,zero) sep_algebra
+begin
+definition zero_vec_def: "0 \<equiv> (0,0)"
+end
+
+
+end
