Sep_Algebra_Vector.thy
@@ -1,0 +1,10 @@
+theory Sep_Algebra_Vector
+imports  QHLProver.Partial_State Actions.Sep_Prod_Instance QHLProver.Partial_State
+begin                                      
+instantiation vec :: (comm_ring_1) sep_algebra
+begin
+definition zero_vec_def: "0 \<equiv> dim_vec "
+end
+
+
+end
